Remove PulseSyntaxExtension.SyntaxWrapper module
Replace the ML-backed SyntaxWrapper abstraction layer with direct
Pulse.Syntax.* module calls. The syntax extension now includes the
checker source (src/checker) and references Pulse.Syntax.{Base,Pure,
Builder,Naming} directly.

Key changes:
- Delete PulseSyntaxExtension.SyntaxWrapper.fsti (168 lines)
- Delete PulseSyntaxExtension_SyntaxWrapper.ml (277 lines)
- Replace ~130 SW.* references in Desugar.fst with direct calls
- Add coerce helper (using coerce_eq + admit) to bridge the
  FStarC.Syntax.Syntax.term / FStar.Stubs.Reflection.Types.term
  type distinction (same at OCaml level, different in F*)
- Update build system: syntax_extension now depends on checker
- Add local ASTBuilder.fsti for syntax_extension build context
- Update Printing.fst to construct emp_inames directly

Co-authored-by: Copilot <223556219+Copilot@users.noreply.github.com>

pulse/src/syntax_extension/PulseSyntaxExtension.Desugar.fst
@@ -42,142 +42,148 @@ open PulseSyntaxExtension.Err
 open PulseSyntaxExtension.Env
 
 (* Helper functions replacing PulseSyntaxExtension.SyntaxWrapper *)
+
+(* FStarC.Syntax.Syntax.term and Pulse.Syntax.Base.term (= FStar.Stubs.Reflection.Types.term)
+   are the same type at the OCaml level but different in F*. Since we build with --lax,
+   we use coerce_eq with admit() to bridge them. coerce_eq extracts as the identity. *)
+let coerce (#a #b : Type) (x:a) : b = FStar.Pervasives.coerce_eq (admit()) x
+
 let ppname_of_id (i:ident) : ppname =
-  mk_ppname (RT.seal_pp_name (Ident.string_of_id i)) (Ident.range_of_id i)
+  mk_ppname (RT.seal_pp_name (Ident.string_of_id i)) (coerce (Ident.range_of_id i))
 
 let sw_mk_binder (x:ident) (t:term) : binder =
-  mk_binder_ppname t (ppname_of_id x)
+  mk_binder_ppname (coerce t) (ppname_of_id x)
 
 let sw_mk_binder_with_attrs (x:ident) (t:term) (attrs:list term) : binder =
-  Pulse.Syntax.Base.mk_binder_with_attrs t (ppname_of_id x) (FStar.Sealed.seal attrs)
+  Pulse.Syntax.Base.mk_binder_with_attrs (coerce t) (ppname_of_id x) (FStar.Sealed.seal (coerce attrs))
 
-let sw_mk_bv (i:index) (name:string) (r:FStarC.Range.range) : bv =
-  { bv_index = i; bv_ppname = mk_ppname (RT.seal_pp_name name) r }
+let sw_mk_bv (i:Pulse.Syntax.Base.index) (name:string) (r:FStarC.Range.range) : bv =
+  { bv_index = i; bv_ppname = mk_ppname (RT.seal_pp_name name) (coerce r) }
 
-let sw_mk_fv (nm:lident) (r:FStarC.Range.range) : fv =
-  { fv_name = Ident.path_of_lid nm; fv_range = r }
+let sw_mk_fv (nm:lident) (r:FStarC.Range.range) : ML fv =
+  { fv_name = Ident.path_of_lid nm; fv_range = coerce r }
 
-let as_qual (imp:bool) : option qualifier = if imp then Some Implicit else None
+let sw_as_qual (imp:bool) : option qualifier = if imp then Some Implicit else None
 let tc_qual : option qualifier = Some TcArg
-let meta_qual (t:term) : option qualifier = Some (Meta t)
+let meta_qual (t:term) : option qualifier = Some (Meta (coerce t))
 
-let tm_emp (r:FStarC.Range.range) : term = PSP.pack_term_view PSP.Tm_Emp r
-let tm_pure (p:term) (r:FStarC.Range.range) : term = PSP.pack_term_view (PSP.Tm_Pure p) r
-let tm_unknown (r:FStarC.Range.range) : term = PSP.pack_term_view PSP.Tm_Unknown r
-let tm_expr (t:S.term) (r:FStarC.Range.range) : term = PSP.wr t r
+let tm_emp (r:FStarC.Range.range) : term = coerce (PSP.pack_term_view PSP.Tm_Emp (coerce r))
+let tm_pure (p:term) (r:FStarC.Range.range) : term = coerce (PSP.pack_term_view (PSP.Tm_Pure (coerce p)) (coerce r))
+let tm_unknown (r:FStarC.Range.range) : term = coerce (PSP.pack_term_view PSP.Tm_Unknown (coerce r))
+let tm_expr (t:S.term) (r:FStarC.Range.range) : term = coerce (PSP.wr (coerce t) (coerce r))
 
 let sw_mk_st_comp (pre:term) (ret:binder) (post:term) : st_comp =
-  { u = PSP.u_unknown; res = ret.binder_ty; pre; post }
+  { u = PSP.u_unknown; res = coerce ret.binder_ty; pre = coerce pre; post = coerce post }
 
-let mk_comp (pre:term) (ret:binder) (post:term) : comp =
+let sw_mk_comp (pre:term) (ret:binder) (post:term) : comp =
   C_ST (sw_mk_st_comp pre ret post)
 
 let ghost_comp (opens:term) (pre:term) (ret:binder) (post:term) : comp =
-  C_STGhost opens (sw_mk_st_comp pre ret post)
+  C_STGhost (coerce opens) (sw_mk_st_comp pre ret post)
 
 let atomic_comp (opens:term) (pre:term) (ret:binder) (post:term) : comp =
-  C_STAtomic opens Observable (sw_mk_st_comp pre ret post)
+  C_STAtomic (coerce opens) Observable (sw_mk_st_comp pre ret post)
 
 let unobs_comp (opens:term) (pre:term) (ret:binder) (post:term) : comp =
-  C_STAtomic opens Neutral (sw_mk_st_comp pre ret post)
+  C_STAtomic (coerce opens) Neutral (sw_mk_st_comp pre ret post)
 
-let mk_tot (t:term) : comp = C_Tot t
+let mk_tot (t:term) : comp = C_Tot (coerce t)
 
 let tm_return (t:term) (r:FStarC.Range.range) : st_term =
-  PSBuild.(with_range (tm_return PSP.tm_unknown false t) r)
+  coerce (PSBuild.(with_range (tm_return PSP.tm_unknown false (coerce t)) (coerce r)))
 
 let tm_ghost_return (t:term) (r:FStarC.Range.range) : st_term =
-  PSBuild.(with_range (tm_return PSP.tm_unknown false t) r)
+  coerce (PSBuild.(with_range (tm_return PSP.tm_unknown false (coerce t)) (coerce r)))
 
 let tm_abs (b:binder) (q:option qualifier) (c:option comp) (body:st_term) (r:FStarC.Range.range) : st_term =
-  let asc = { annotated = c; elaborated = None } in
-  PSBuild.(with_range (tm_abs b q asc body) r)
+  let asc : comp_ascription = coerce { annotated = c; elaborated = None } in
+  coerce (PSBuild.(with_range (tm_abs (coerce b) (coerce q) asc (coerce body)) (coerce r)))
 
 let tm_st (head:term) (args:list st_term) (r:FStarC.Range.range) : st_term =
-  PSBuild.(with_range (tm_st head args) r)
+  coerce (PSBuild.(with_range (tm_st (coerce head) (coerce args)) (coerce r)))
 
 let tm_bind (x:binder) (e1:st_term) (e2:st_term) (r:FStarC.Range.range) : st_term =
-  PSBuild.(with_range (tm_bind x e1 e2) r)
+  coerce (PSBuild.(with_range (tm_bind (coerce x) (coerce e1) (coerce e2)) (coerce r)))
 
 let tm_totbind (x:binder) (e1:term) (e2:st_term) (r:FStarC.Range.range) : st_term =
-  PSBuild.(with_range (tm_totbind x e1 e2) r)
+  coerce (PSBuild.(with_range (tm_totbind (coerce x) (coerce e1) (coerce e2)) (coerce r)))
 
 let tm_let_mut (x:binder) (v:option term) (k:st_term) (r:FStarC.Range.range) : st_term =
-  PSBuild.(with_range (tm_with_local x v k) r)
+  coerce (PSBuild.(with_range (tm_with_local (coerce x) (coerce v) (coerce k)) (coerce r)))
 
 let tm_let_mut_array (x:binder) (v:option term) (n:term) (k:st_term) (r:FStarC.Range.range) : st_term =
-  PSBuild.(with_range (tm_with_local_array x v n k) r)
+  coerce (PSBuild.(with_range (tm_with_local_array (coerce x) (coerce v) (coerce n) (coerce k)) (coerce r)))
 
 let tm_while (head:st_term) (invariant:slprop) (body:st_term) (loop_requires:term) (meas:list term) (r:FStarC.Range.range) : st_term =
-  PSBuild.(with_range (tm_while invariant head body loop_requires meas) r)
+  coerce (PSBuild.(with_range (tm_while (coerce invariant) (coerce head) (coerce body) (coerce loop_requires) (coerce meas)) (coerce r)))
 
 let tm_if (head:st_term) (returns_annot:option slprop) (then_ else_:st_term) (r:FStarC.Range.range) : st_term =
-  PSBuild.(with_range (tm_if head then_ else_ returns_annot) r)
+  coerce (PSBuild.(with_range (tm_if (coerce head) (coerce then_) (coerce else_) (coerce returns_annot)) (coerce r)))
 
 let tm_match (sc:st_term) (returns_:option slprop) (brs:list branch) (r:FStarC.Range.range) : st_term =
-  PSBuild.(with_range (tm_match sc returns_ brs) r)
+  coerce (PSBuild.(with_range (tm_match (coerce sc) (coerce returns_) (coerce brs)) (coerce r)))
 
 let tm_intro_exists (p:slprop) (witnesses:list term) (r:FStarC.Range.range) : st_term =
-  PSBuild.(with_range (tm_intro_exists p witnesses) r)
+  coerce (PSBuild.(with_range (tm_intro_exists (coerce p) (coerce witnesses)) (coerce r)))
 
 let tm_with_options (options:string) (body:st_term) (r:FStarC.Range.range) : st_term =
-  PSBuild.(with_range (tm_pragma_with_options options body) r)
+  coerce (PSBuild.(with_range (tm_pragma_with_options options (coerce body)) (coerce r)))
 
 let tm_forward_jump_label (body:st_term) (lbl:ident) (post:comp) (r:FStarC.Range.range) : st_term =
-  PSBuild.(with_range (tm_forward_jump_label body (ppname_of_id lbl) post) r)
+  coerce (PSBuild.(with_range (tm_forward_jump_label (coerce body) (ppname_of_id lbl) (coerce post)) (coerce r)))
 
 let tm_goto (lbl:term) (arg:term) (r:FStarC.Range.range) : st_term =
-  PSBuild.(with_range (tm_goto lbl arg) r)
+  coerce (PSBuild.(with_range (tm_goto (coerce lbl) (coerce arg)) (coerce r)))
 
 let tm_defer (handler_pre:term) (handler:st_term) (body:st_term) (r:FStarC.Range.range) : st_term =
-  PSBuild.(with_range (tm_defer handler_pre handler body) r)
+  coerce (PSBuild.(with_range (tm_defer (coerce handler_pre) (coerce handler) (coerce body)) (coerce r)))
 
 let tm_admit (r:FStarC.Range.range) : st_term =
-  PSBuild.(with_range (tm_admit STT PSP.u_zero (PSP.pack_term_view PSP.Tm_Unknown r) None) r)
+  coerce (PSBuild.(with_range (tm_admit STT PSP.u_zero (PSP.pack_term_view PSP.Tm_Unknown (coerce r)) None) (coerce r)))
 
 let tm_proof_hint_with_binders (ht:proof_hint_type) (binders:list binder) (s:st_term) (r:FStarC.Range.range) : st_term =
-  PSBuild.with_range (Tm_ProofHintWithBinders { hint_type=ht; binders; t=s }) r
+  coerce (PSBuild.with_range (Tm_ProofHintWithBinders { hint_type=coerce ht; binders=coerce binders; t=coerce s }) (coerce r))
 
-let mk_assert_hint_type = PSBuild.mk_assert_hint_type
-let mk_unfold_hint_type = PSBuild.mk_unfold_hint_type
-let mk_fold_hint_type = PSBuild.mk_fold_hint_type
-let mk_rename_hint_type = PSBuild.mk_rename_hint_type
-let mk_rewrite_hint_type = PSBuild.mk_rewrite_hint_type
+let mk_assert_hint_type (p:slprop) : proof_hint_type = coerce (PSBuild.mk_assert_hint_type (coerce p))
+let mk_unfold_hint_type ns p : proof_hint_type = coerce (PSBuild.mk_unfold_hint_type ns (coerce p))
+let mk_fold_hint_type ns p : proof_hint_type = coerce (PSBuild.mk_fold_hint_type ns (coerce p))
+let mk_rename_hint_type pairs goal tac_opt : proof_hint_type = coerce (PSBuild.mk_rename_hint_type (coerce pairs) (coerce goal) (coerce tac_opt))
+let mk_rewrite_hint_type t1 t2 tac_opt : proof_hint_type = coerce (PSBuild.mk_rewrite_hint_type (coerce t1) (coerce t2) (coerce tac_opt))
 let mk_wild_hint_type : proof_hint_type = WILD
-let mk_show_proof_state_hint_type (r:FStarC.Range.range) : proof_hint_type = SHOW_PROOF_STATE r
+let mk_show_proof_state_hint_type (r:FStarC.Range.range) : proof_hint_type = SHOW_PROOF_STATE (coerce r)
 
-let inspect_const (c:FStarC.Const.sconst) : constant =
-  FStarC.Reflection.V2.Builtins.inspect_const c
+let inspect_const (c:FStarC.Const.sconst) : ML constant =
+  coerce (FStarC.Reflection.V2.Builtins.inspect_const c)
 
-let pat_var (s:string) (_r:FStarC.Range.range) : pattern = Pat_Var (RT.seal_pp_name s) S.tun
+let pat_var (s:string) (_r:FStarC.Range.range) : pattern = Pat_Var (RT.seal_pp_name s) (coerce S.tun)
 let pat_constant (c:constant) (_r:FStarC.Range.range) : pattern = Pat_Constant c
-let pat_cons (hd:fv) (ps:list pattern) (_r:FStarC.Range.range) : pattern =
+let pat_cons (hd:fv) (ps:list pattern) (_r:FStarC.Range.range) : ML pattern =
   Pat_Cons hd (L.map (fun v -> (v, false)) ps)
 
-let mk_branch (p:pattern) (t:st_term) (norw:bool) : branch = PSBuild.mk_branch p t norw
+let mk_branch (p:pattern) (t:st_term) (norw:bool) : branch = coerce (PSBuild.mk_branch (coerce p) (coerce t) (coerce norw))
 
-let bvs_as_subst (vars:list var) : PSN.subst =
+let bvs_as_subst (vars:list var) : ML PSN.subst =
   L.fold_left
     (fun s b -> RT.ND b 0 :: PSN.shift_subst s)
     [] vars
 
-let subst_st_term (s:PSN.subst) (t:st_term) : st_term = PSN.subst_st_term t s
-let subst_proof_hint (s:PSN.subst) (h:proof_hint_type) : proof_hint_type = PSN.subst_proof_hint h s
+let subst_st_term (s:PSN.subst) (t:st_term) : st_term = coerce (PSN.subst_st_term (coerce t) s)
+let subst_proof_hint (s:PSN.subst) (h:proof_hint_type) : proof_hint_type = coerce (PSN.subst_proof_hint (coerce h) s)
 
-let fn_defn rng id isrec us bs comp meas body : decl =
-  PSBuild.mk_decl (PSBuild.mk_fn_defn id isrec us bs comp meas body) rng
-let fn_decl rng id us bs comp : decl =
-  PSBuild.mk_decl (PSBuild.mk_fn_decl id us bs comp) rng
+let fn_defn rng id isrec us bs (comp:Pulse.Syntax.Base.comp) meas body : decl =
+  coerce (PSBuild.mk_decl (coerce (PSBuild.mk_fn_defn (coerce id) isrec (coerce us) (coerce bs) (coerce comp) (coerce meas) (coerce body))) (coerce rng))
+let fn_decl rng id us bs (comp:Pulse.Syntax.Base.comp) : decl =
+  coerce (PSBuild.mk_decl (coerce (PSBuild.mk_fn_decl (coerce id) (coerce us) (coerce bs) (coerce comp))) (coerce rng))
 let slprop_defn rng id bs body : decl =
-  PSBuild.mk_decl (PSBuild.mk_slprop_defn id bs body) rng
+  coerce (PSBuild.mk_decl (coerce (PSBuild.mk_slprop_defn (coerce id) (coerce bs) (coerce body))) (coerce rng))
 
 assume val print_exn (e:exn) : string
 
 let close_st_term_bvs (e:st_term) (xs:list bv) : ML st_term = 
-  PSN.close_st_term_n e (L.map (fun (b:bv) -> b.bv_index) xs)
+  coerce (PSN.close_st_term_n (coerce e) (L.map (fun (b:bv) -> b.bv_index) xs))
 
 let close_comp_bvs  (e:comp) (xs:list bv) : ML comp = 
-  PSN.close_comp_n e (L.map (fun (b:bv) -> b.bv_index) xs)
+  coerce (PSN.close_comp_n (coerce e) (L.map (fun (b:bv) -> b.bv_index) xs))
 
 
 let rec fold_right1 (f : 'a -> 'a -> ML 'a) (l : list 'a) : ML 'a =
@@ -278,7 +284,7 @@ let as_term (t:S.term)
     | _ -> 
       tm_expr t t.pos
 
-let desugar_const (c:FStarC.Const.sconst) : constant =
+let desugar_const (c:FStarC.Const.sconst) : ML constant =
   inspect_const c
 
 let comp_to_ast_term (c:Sugar.computation_type) : ML (err A.term) =
@@ -425,7 +431,7 @@ let idents_as_binders (env:env_t) (l:list ident)
           | [] -> return (env, L.rev binders, L.rev bvs)
           | i::l ->
             let env, bv = push_bv env i in
-            let qual = as_qual true in      
+            let qual = sw_as_qual true in      
             let ty = mk_ty i in
             let! ty = desugar_term env ty in
             aux env ((qual, sw_mk_binder i ty)::binders) (bv::bvs) l
@@ -433,17 +439,18 @@ let idents_as_binders (env:env_t) (l:list ident)
       aux env [] [] l
 
 let desugar_slprop (env:env_t) (v:Sugar.slprop)
-  : ML (err slprop)
-  = tosyntax env v
+  : ML (err term)
+  = let! t = tosyntax env v in
+    return (coerce t)
 
 let desugar_slprop_annot (env:env_t) (v:Sugar.slprop) (lit:bool)
-  : ML (err slprop)
+  : ML (err term)
   = let! p = tosyntax env v in
     if lit then
-      return <| U.mk_app (S.tconst (FStarC.Parser.Const.p2l ["Pulse"; "Lib"; "Core"; "literally"]))
-        [p, None]
+      return (coerce (U.mk_app (S.tconst (FStarC.Parser.Const.p2l ["Pulse"; "Lib"; "Core"; "literally"]))
+        [p, None]))
     else
-      return p
+      return (coerce p)
 
 let desugar_computation_type (env:env_t) (c:Sugar.computation_type)
   : ML (err comp)
@@ -457,7 +464,7 @@ let desugar_computation_type (env:env_t) (c:Sugar.computation_type)
     let! opens =
       match annots.Sugar.opens with
       | Some t -> desugar_term env t
-      | None -> return PSP.tm_emp_inames
+      | None -> return (coerce PSP.tm_emp_inames)
     in
 
     (* Should have return_name in scope I think *)
@@ -468,7 +475,7 @@ let desugar_computation_type (env:env_t) (c:Sugar.computation_type)
     // let! posts = map_err (desugar_slprop env1) c.postconditions in
     // let post = fold_right1 (fun a b -> tm_star a b c.range) posts in
     let! post = desugar_slprop_annot env1 annots.Sugar.postcondition c.literally in
-    let post = PSN.close_term post bv.index in
+    let post = coerce (PSN.close_term (coerce post) bv.index) in
 
     match c.tag with
     | Sugar.ST ->
@@ -476,7 +483,7 @@ let desugar_computation_type (env:env_t) (c:Sugar.computation_type)
         fail "STT computations are not indexed by invariants. Either remove the `opens` or make this function ghost/atomic."
              (Some?.v annots.Sugar.opens).range
       else return ();!
-      return (mk_comp pre (sw_mk_binder annots.Sugar.return_name ret) post)
+      return (sw_mk_comp pre (sw_mk_binder annots.Sugar.return_name ret) post)
     | Sugar.STAtomic ->
       return (atomic_comp opens pre (sw_mk_binder annots.Sugar.return_name ret) post)
     | Sugar.STUnobservable ->
@@ -559,11 +566,11 @@ let mk_abs_with_comp qbs comp body range : ML _ =
   let _, abs =
     L.fold_right
       (fun (q,b,bv) (c, body) ->
-        let body' = PSN.close_st_term body bv.bv_index in
+        let body' = coerce (PSN.close_st_term (coerce body) bv.bv_index) in
         let asc =
           match c with
           | None -> None
-          | Some c -> Some  (PSN.close_comp c bv.bv_index) in
+          | Some c -> Some  (coerce (PSN.close_comp (coerce c) bv.bv_index)) in
         None, tm_abs b q asc body' range)
       qbs (comp, body)
   in
@@ -580,7 +587,7 @@ let rec desugar_stmt' (env:env_t) (s:Sugar.stmt)
         return (st_term_of_admit_or_return (admit_or_return env tm))
       else (
         let! args = desugar_st_args env args in
-        return (tm_st tm args s.range)
+        return (tm_st (coerce tm) args s.range)
       )
 
     | ArrayAssignment { arr; index; value } ->
@@ -748,16 +755,16 @@ let rec desugar_stmt' (env:env_t) (s:Sugar.stmt)
         | _ -> mapM (tosyntax env) meas_list
       in
 
-      let while = tm_while guard inv body loop_requires meas s.range in
-      let while = PSN.close_st_term while lblx.index in
+      let while = tm_while guard inv body (coerce loop_requires) (coerce meas) s.range in
+      let while = coerce (PSN.close_st_term (coerce while) lblx.index) in
 
       let loop_ensures = invs0 |> L.concatMap (function | LoopEnsures r -> [r] | _ -> []) in
       let! loop_ensures = mapM (tosyntax env) loop_ensures in
       let loop_ensures =
         match loop_ensures with
         | [] -> tm_emp s.range
-        | r::rs -> tm_pure (L.fold_left U.mk_disj r rs) s.range in
-      let loop_ensures = mk_comp (tm_unknown s.range) (sw_mk_binder (id_of_text "_") (tm_unknown s.range)) loop_ensures in
+        | r::rs -> tm_pure (coerce (L.fold_left U.mk_disj r rs)) s.range in
+      let loop_ensures = sw_mk_comp (tm_unknown s.range) (sw_mk_binder (id_of_text "_") (tm_unknown s.range)) loop_ensures in
       return (tm_forward_jump_label while breaklbl loop_ensures s.range)
 
     | Introduce { slprop; witnesses } -> (
@@ -778,20 +785,20 @@ let rec desugar_stmt' (env:env_t) (s:Sugar.stmt)
     | ForwardJumpLabel { body; lbl; post } ->
       let env', lblx = push_bv env lbl in
       let! body = desugar_stmt env' body in
-      let body = PSN.close_st_term body lblx.index in
+      let body = coerce (PSN.close_st_term (coerce body) lblx.index) in
       let! post =
         match post with
         | None -> return (tm_emp s.range)
         | Some (_, t, _opens) -> desugar_slprop env t
       in
-      let post = mk_comp (tm_unknown s.range) (sw_mk_binder (id_of_text "_") (tm_unknown s.range)) post in
+      let post = sw_mk_comp (tm_unknown s.range) (sw_mk_binder (id_of_text "_") (tm_unknown s.range)) post in
       return (tm_forward_jump_label body lbl post s.range)
 
     | Goto { lbl; arg } ->
       let! lbl = tosyntax env (sugar_var (id_as_lid lbl) s.range) in
       let arg = match arg with Some arg -> arg | None -> sugar_unit_const s.range in
       let! arg = tosyntax env arg in
-      return (tm_goto lbl arg s.range)
+      return (tm_goto (coerce lbl) (coerce arg) s.range)
 
     | Defer { handler_pre; defer_handler } ->
       fail "defer must be followed by a body (use defer pre { handler }; body)" s.range
@@ -816,7 +823,7 @@ and desugar_st_args (env:env_t) (args:list Sugar.lambda) : ML (err (list st_term
 and desugar_stmt (env:env_t) (s:Sugar.stmt) : ML (err st_term) =
   let! r = desugar_stmt' env s in
   if not s.source then
-    return (PSBuild.mark_not_source r)
+    return (coerce (PSBuild.mark_not_source (coerce r)))
   else
     return r
 
@@ -826,7 +833,7 @@ and desugar_branch (env:env_t) (br: bool & A.pattern & Sugar.stmt)
     let! (p, vs) = desugar_pat env p in
     let env, bvs = push_bvs env vs in
     let! e = desugar_stmt env e in
-    let e = PSN.close_st_term_n e (L.map (fun (v:S.bv) -> v.index <: nat) bvs) in
+    let e = coerce (PSN.close_st_term_n (coerce e) (L.map (fun (v:S.bv) -> v.index <: nat) bvs)) in
     return (mk_branch p e norw)
 
 and desugar_pat (env:env_t) (p:A.pattern)
@@ -899,7 +906,7 @@ and desugar_bind (env:env_t) (lb:_) (s2:Sugar.stmt) (r:R.range)
     let! s2 =
       let env, bv = push_bv env id in
       let! s2 = desugar_stmt env s2 in
-      return (PSN.close_st_term s2 bv.index)
+      return (coerce (PSN.close_st_term (coerce s2) bv.index))
     in
     match lb.init with
     | None ->
@@ -965,7 +972,7 @@ and desugar_bind (env:env_t) (lb:_) (s2:Sugar.stmt) (r:R.range)
         | Default_initializer (Some e1, args) ->
           let! s1 = tosyntax env e1 in
           let! args = desugar_st_args env args in
-          let t = mk_bind b (tm_st s1 args r) s2 r in
+          let t = mk_bind b (tm_st (coerce s1) args r) s2 r in
           return t
 
         | Stmt_initializer e ->
@@ -1003,7 +1010,7 @@ and desugar_sequence (env:env_t) (s1 s2:Sugar.stmt) r
     let! s1 = desugar_stmt env s1 in
     let s1 =
       if semicolon
-      then PSBuild.mark_statement_sequence s1
+      then coerce (PSBuild.mark_statement_sequence (coerce s1))
       else s1
     in
     let! s2 = desugar_stmt env s2 in
@@ -1015,9 +1022,9 @@ and desugar_proof_hint_with_binders (env:env_t) (s1:Sugar.stmt) (k:option Sugar.
   = match s1.s with
     | Sugar.ProofHintWithBinders { hint_type = Sugar.ASSUME p; binders=[] } ->
       let assume_fv = sw_mk_fv assume_lid r in
-      let assume_ : term = PSP.tm_fvar assume_fv in
+      let assume_ : term = coerce (PSP.tm_fvar (coerce assume_fv)) in
       let! p = desugar_slprop env p in
-      let s1 = tm_st (S.mk_Tm_app assume_ [p, None] r) [] r in
+      let s1 = tm_st (coerce (S.mk_Tm_app (coerce assume_) [coerce p, None] r)) [] r in
       let! s2 =
         match k with
         | None -> return (tm_ghost_return (tm_expr S.unit_const r) r)
@@ -1040,7 +1047,7 @@ and desugar_proof_hint_with_binders (env:env_t) (s1:Sugar.stmt) (k:option Sugar.
       let sub = bvs_as_subst vars in
       let s2 = subst_st_term sub s2 in
       let ht = subst_proof_hint sub ht in
-      return (tm_proof_hint_with_binders ht (PSN.close_binders binders vars) s2 r)
+      return (tm_proof_hint_with_binders ht (coerce (PSN.close_binders (coerce binders) vars)) s2 r)
     | _ -> fail "Expected ProofHintWithBinders" s1.range
 
 and desugar_binders (env:env_t) (bs:Sugar.binders)
@@ -1087,14 +1094,14 @@ and desugar_lambda (env:env_t) (l:Sugar.lambda)
 
 and as_qual (env:env_t) (q:A.aqual) rng : ML (err qual) =
   match q with
-  | Some A.Implicit -> return <| as_qual true
+  | Some A.Implicit -> return <| sw_as_qual true
   | Some A.TypeClassArg -> return <| tc_qual
   | Some (A.Meta t) ->
     let! t = desugar_term env t in
     return <| meta_qual t
   | Some A.Equality ->
     fail "Pulse does not yet support equality arguments" rng
-  | None -> return <| as_qual false
+  | None -> return <| sw_as_qual false
 
 
 let desugar_decl (env:env_t) (d:Sugar.decl)
@@ -1129,14 +1136,14 @@ let desugar_decl (env:env_t) (d:Sugar.decl)
   // A (non-recursive) definition where the body is a lambda.
   | Sugar.FnDefn { id; is_rec=false; us; binders; ascription=Inr ascription; measure=None; body=Inr body; range } ->
     let! env, bs, bvs = desugar_binders env binders in
-    let! comp = 
+    let! cmp = 
       match ascription with
       | None -> return (mk_tot (tm_unknown range))
       | Some t -> let! t = desugar_term env t in return (mk_tot t)
     in
     let! body = desugar_lambda env body in
     let! qbs = map2 faux bs bvs in
-    return (fn_defn range id false us qbs comp None body)
+    return (fn_defn range id false us qbs cmp (None #term) body)
 
   // A recursive definition where the body is a lambda, not supported yet.
   | Sugar.FnDefn { id; is_rec=true; us; binders; ascription=Inr ascription; measure=None; body=Inr body; range } ->
